extraction/Encoding.ml
@@ -1,0 +1,122 @@
+type codepoint = int
+
+module Utf8Utils = struct
+  let from_int (u: int) : char list =
+    match u with
+    | u when u < 0 -> assert false
+    | u when u <= 0x007F -> Char.chr u :: []
+    | u when u <= 0x07FF -> Char.chr (0xC0 lor (u lsr 6)) :: Char.chr (0x80 lor (u land 0x3F)) :: []
+    | u when u <= 0xFFFF -> Char.chr (0xE0 lor (u lsr 12)) :: Char.chr (0x80 lor ((u lsr 6) land 0x3F)) :: Char.chr (0x80 lor (u land 0x3F)) :: []
+    | u when u <= 0x10FFFF -> Char.chr (0xF0 lor (u lsr 18)) :: Char.chr (0x80 lor ((u lsr 12) land 0x3F)) :: Char.chr (0x80 lor ((u lsr 6) land 0x3F)) :: Char.chr (0x80 lor (u land 0x3F)) :: []
+    | _ -> failwith "Int is to big for a unicode character!"
+
+    
+    let is_high_surrogate (c: int) = (0xd800 <= c) && (c <= 0xdbff)
+    let is_low_surrogate (c: int) = (0xdc00 <= c) && (c <= 0xdfff)
+    (* I.e. not a surrogate *)
+    let is_normal (c: int) = (0x0000 <= c && c < 0xd800) || (0xe000 <= c)
+
+    let replacement_int = 0xFFFD
+    let replacement_uchar = Uchar.of_int replacement_int
+end
+
+module type Character = sig
+  type character
+
+  val cmp: character -> character -> int
+
+  val chars_from_int: int -> character list
+  val char_from_int: int -> character
+  val char_to_int: character -> int
+
+  val list_from_string: string -> character list
+  val list_to_string: character list -> string
+end
+
+module Utf16 : Character with type character = Unsigned.UInt16.t = struct
+  type character = Unsigned.UInt16.t
+  let cmp (l: character) (r: character): int = Unsigned.UInt16.compare l r
+
+  let chars_from_int (code: int) : character list = 
+    if code > 0xFFFF then
+      (let shifted = (code - 0x10000) in
+      let high = (shifted / 0x400) + 0xd800 in
+      let low = (shifted mod 0x400) + 0xdc0 in
+      (Unsigned.UInt16.of_int high) :: (Unsigned.UInt16.of_int low) :: [])
+    else
+      (Unsigned.UInt16.of_int code) :: []
+
+  let char_from_int c = Utils.List.unique (chars_from_int c)
+
+  let char_to_int (c: character) = Unsigned.UInt16.to_int c
+
+  (* let clean_utf16 (str: Unsigned.uint16 list) = 
+    let rec iter (str: int list) =
+      match str with
+      | h :: l :: t when Utf8Utils.is_high_surrogate h && Utf8Utils.is_low_surrogate l -> (
+        (Unsigned.UInt16.of_int h) :: (Unsigned.UInt16.of_int l) :: (iter t)
+      )
+      | h :: t when Utf8Utils.is_normal h -> (Unsigned.UInt16.of_int h) :: (iter t)
+      | _ :: t -> (Unsigned.UInt16.of_int 0xFFFD) :: (iter t)
+      | [] -> []
+    in
+    iter (List.map Unsigned.UInt16.to_int str) *)
+
+  let list_from_string (str: string): character list = 
+    let is = List.init (String.length str) (fun i -> i) in
+    Utils.List.flat_map (fun i ->
+      let u = StringLabels.get_utf_8_uchar str i in
+      if Uchar.utf_decode_is_valid u then
+        chars_from_int (Uchar.to_int (Uchar.utf_decode_uchar u))
+      else
+        []
+    ) is
+
+  let list_to_string (str: character list): string = 
+    let b = Buffer.create (List.length str) in
+    let rec iter (str: int list) =
+      match str with
+      | h :: l :: t when Utf8Utils.is_high_surrogate h && Utf8Utils.is_low_surrogate l -> (
+        let i = 0x10000 + (h - 0xd800)*0x400 + (l - 0xdc00) in
+        assert (Utf8Utils.is_normal i);
+        Buffer.add_utf_8_uchar b (Uchar.of_int i);
+        iter t
+      )
+      | h :: t when Utf8Utils.is_normal h -> Buffer.add_utf_8_uchar b (Uchar.of_int h); iter t
+      | _ :: t -> Buffer.add_utf_8_uchar b (Uchar.of_int 0xFFFD); iter t
+      | [] -> ()
+    in
+    iter (List.map Unsigned.UInt16.to_int str);
+    Buffer.contents b 
+end
+
+module Unicode : Character with type character = int = struct
+  type character = int
+  let cmp (l: character) (r: character): int = Int.compare l r
+
+  let chars_from_int (code: int) : character list = code :: []
+
+  let char_from_int c = Utils.List.unique (chars_from_int c)
+
+  let char_to_int (c: character) = c
+
+  let list_from_string (str: string): character list = 
+    let is = List.init (String.length str) (fun i -> i) in
+    Utils.List.flat_map (fun i ->
+      let u = StringLabels.get_utf_8_uchar str i in
+      if Uchar.utf_decode_is_valid u then
+        (Uchar.to_int (Uchar.utf_decode_uchar u)) :: []
+      else
+        []
+    ) is
+
+    let list_to_string (str: character list): string = 
+      let b = Buffer.create (List.length str) in
+      List.iter ( fun c ->
+        if Uchar.is_valid c then
+          Buffer.add_utf_8_uchar b (Uchar.of_int c)
+        else
+          Buffer.add_utf_8_uchar b Utf8Utils.replacement_uchar
+      ) str;
+      Buffer.contents b 
+end
