extraction/Engines.ml
@@ -1,0 +1,26 @@
+open Extracted
+
+module type Engine = sig
+  include Encoding.Character
+
+  val countGroups: character Patterns.coq_Regex -> int
+
+  val compilePattern :
+    character Patterns.coq_Regex -> RegExpRecord.coq_type ->
+    (character list -> non_neg_integer -> character
+    Notation.coq_MatchResult, CompileError.coq_type) Result.coq_Result
+ end
+
+module Utf16Engine : Engine
+  with type character = Unsigned.uint16
+= struct
+  include Encoding.Utf16
+  include Extracted.ECMA
+end
+
+module UnicodeEngine : Engine
+  with type character = int
+= struct
+  include Encoding.Unicode
+  include Extracted.ECMA_u
+end
