extraction/Interop.ml
@@ -1,33 +1,25 @@
-exception NotImplemented of string
+module Common = struct
+  let parse_hex ls =
+    int_of_string ("0x" ^ (String.concat "" (List.map (fun c -> String.make 1 c) ls)))
 
-let parse_hex ls =
-  int_of_string ("0x" ^ (String.concat "" (List.map (fun c -> String.make 1 c) ls)))
+  let digits: char list = '0' :: '1' :: '2' :: '3' :: '4' :: '5' :: '6' :: '7' :: '8' :: '9' :: []
 
-module Utf16 = struct
-  type character = Unsigned.uint16
-  let char_eq (l: character) (r: character) = Unsigned.UInt16.equal l r
-  let char_to_int (c: character): int = Unsigned.UInt16.to_int c
-  let char_of_int (i: int): character = Unsigned.UInt16.of_int i
-  let cmp (l: character) (r: character): int = Unsigned.UInt16.compare l r
+  let ascii_word_characters: char list =
+    let str = "ABCDEFGHIJKLMNOPQRSTUVWXYZabcdefghijklmnopqrstuvwxyz0123456789_" in
+    List.init (String.length str) (String.get str)
 
-
-  let to_character_list (ls: char list): character list = List.map (fun c -> char_of_int (Char.code c)) ls
-  let all_chars: character list = 
-      List.init (Unsigned.UInt16.to_int Unsigned.UInt16.max_int) (fun i -> i)
-        |> List.map char_of_int
-
-  let line_terminators: character list = (List.map (char_of_int) ( 
+  let line_terminators: int list =
     0x000A :: (* <LF> *)
     0x000D :: (* <CR> *)
     0x2028 :: (* <LS> *)
     0x2029 :: (* <PS> *)
-    []))
-  let white_spaces: character list = (List.map (char_of_int) ( 
+    []
+
+  let white_spaces: int list =
     9 :: (* <TAB> *)
     11 :: (* <VT> *)
     12 :: (* <FF> *)
     32 :: 
-    (* 133 ::  *)
     160 :: 
     5760 ::
     8192 ::
@@ -45,164 +37,13 @@ module Utf16 = struct
     8239 ::
     8287 ::
     12288 ::
-    []))
-  let digits: character list = to_character_list ('0' :: '1' :: '2' :: '3' :: '4' :: '5' :: '6' :: '7' :: '8' :: '9' :: [])
-  let ascii_word_characters: character list = to_character_list (
-    let str = "ABCDEFGHIJKLMNOPQRSTUVWXYZabcdefghijklmnopqrstuvwxyz0123456789_" in
-    List.init (String.length str) (String.get str))
+    []
 
-  let codepoint_to_utf16 (code: int) : Unsigned.uint16 list = 
-    if code > 0xFFFF then
-      (let shifted = (code - 0x10000) in
-      let high = (shifted / 0x400) + 0xd800 in
-      let low = (shifted mod 0x400) + 0xdc0 in
-      (Unsigned.UInt16.of_int high) :: (Unsigned.UInt16.of_int low) :: [])
-    else
-      (Unsigned.UInt16.of_int code) :: []
-
-  let uchar_to_utf16 (u: Uchar.t) : Unsigned.uint16 list = 
-    codepoint_to_utf16 (Uchar.to_int u)
-
-  let string_to_utf16 (str: string): Unsigned.uint16 list = 
-    let is = List.init (String.length str) (fun i -> i) in
-    let ls = List.map (fun i ->
-      let u = StringLabels.get_utf_8_uchar str i in
-      if Uchar.utf_decode_is_valid u then
-        uchar_to_utf16 (Uchar.utf_decode_uchar u)
-      else
-        []
-    ) is in
-    List.flatten ls
-
-  let to_utf8 u: bytes =
-    let rec iter u: int list =
-      match u with
-      | u when u < 0 -> assert false
-      | u when u <= 0x007F -> u :: []
-      | u when u <= 0x07FF -> (0xC0 lor (u lsr 6)) :: (0x80 lor (u land 0x3F)) :: []
-      | u when u <= 0xFFFF -> (0xE0 lor (u lsr 12)) :: (0x80 lor ((u lsr 6) land 0x3F)) :: (0x80 lor (u land 0x3F)):: []
-      | u when u <= 0x10FFFF -> (0xF0 lor (u lsr 18)) :: (0x80 lor ((u lsr 12) land 0x3F)) :: (0x80 lor ((u lsr 6) land 0x3F)) :: (0x80 lor (u land 0x3F)):: []
-      | _ -> assert false
-    in
-    let ls = iter u in
-    Bytes.init (List.length ls) (fun i -> Char.chr (List.nth ls i))
-
-  let clean_utf16 (str: Unsigned.uint16 list) = 
-    let is_high c = (0xd800 <= c) && (c <= 0xdbff) in
-    let is_low c = (0xdc00 <= c) && (c <= 0xdfff) in
-    let is_normal c = (0x0000 <= c && c < 0xd800) || (0xe000 <= c) in (* (Bool.not (is_high c)) && (Bool.not (is_low c)) in *)
-    let rec iter (str: int list) =
-      match str with
-      | h :: l :: t when is_high h && is_low l -> (
-        (Unsigned.UInt16.of_int h) :: (Unsigned.UInt16.of_int l) :: (iter t)
-      )
-      | h :: t when is_normal h -> (Unsigned.UInt16.of_int h) :: (iter t)
-      | _ :: t -> (Unsigned.UInt16.of_int 0xFFFD) :: (iter t)
-      | [] -> []
-    in
-    iter (List.map Unsigned.UInt16.to_int str)
-
-  let utf16_to_string (str: Unsigned.uint16 list) = 
-    let is_high c = (0xd800 <= c) && (c <= 0xdbff) in
-    let is_low c = (0xdc00 <= c) && (c <= 0xdfff) in
-    let is_normal c = (0x0000 <= c && c < 0xd800) || (0xe000 <= c) in (* (Bool.not (is_high c)) && (Bool.not (is_low c)) in *)
-    let b = Buffer.create (List.length str) in
-    let rec iter (str: int list) =
-      match str with
-      | h :: l :: t when is_high h && is_low l -> (
-        let i = 0x10000 + (h - 0xd800)*0x400 + (l - 0xdc00) in
-        assert (is_normal i);
-        Buffer.add_utf_8_uchar b (Uchar.of_int i);
-        iter t
-      )
-      | h :: t when is_normal h -> Buffer.add_utf_8_uchar b (Uchar.of_int h); iter t
-      | _ :: t -> Buffer.add_utf_8_uchar b (Uchar.of_int 0xFFFD); iter t
-      | [] -> ()
-    in
-    iter (List.map Unsigned.UInt16.to_int str);
-    Buffer.contents b 
-
-  type codepoint = int
-  let numeric_value (c: codepoint): int = c
-  let ascii_letter (c: char): codepoint = Char.code c
-  let code_point (c: character): codepoint = char_to_int c
-
-  let to_upper_case (c: codepoint): codepoint list =
-      if Uchar.is_valid c then
-        match Uucp.Case.Map.to_upper (Uchar.of_int c) with
-          | `Self -> c :: []
-          | `Uchars ls -> List.map Uchar.to_int ls
-      else c :: []
-    
-
-  (* The two following functions perform conversions from codepoint to character; should they? *)
-  let code_points_to_string (c: codepoint list): character list = List.flatten (List.map codepoint_to_utf16 c)
+  let list_flat_map (type a b) (f: a -> b list) (ls: a list): b list =
+    List.flatten (List.map f ls)
 end
 
-module Unicode = struct
-  let string_to_utf8 (str: string): int list = 
-    let is = List.init (String.length str) (fun i -> i) in
-    List.map (fun i ->
-      let u = StringLabels.get_utf_8_uchar str i in
-      if Uchar.utf_decode_is_valid u then
-        Uchar.to_int (Uchar.utf_decode_uchar u)
-      else
-        0xFFFD
-    ) is
-
-  type character = int
-  let char_eq (l: character) (r: character) = Int.equal l r
-  let char_to_int (c: character): int = c
-  let char_of_int (i: int): character = i
-  let cmp (l: character) (r: character): int = Int.compare l r
-
-  let to_character_list (ls: char list): character list = List.map (fun c -> char_of_int (Char.code c)) ls
-  let all_chars: character list = 
-      List.init (0x10FFFF + 1) (fun i -> i)
-        |> List.map char_of_int
-
-  let line_terminators: character list = (List.map (char_of_int) ( 
-    0x000A :: (* <LF> *)
-    0x000D :: (* <CR> *)
-    0x2028 :: (* <LS> *)
-    0x2029 :: (* <PS> *)
-    []))
-  let white_spaces: character list = (List.map (char_of_int) ( 
-    9 :: (* <TAB> *)
-    11 :: (* <VT> *)
-    12 :: (* <FF> *)
-    32 :: 
-    160 :: 
-    5760 ::
-    8192 ::
-    8193 ::
-    8194 ::
-    8195 ::
-    8196 ::
-    8197 ::
-    8198 ::
-    8199 ::
-    8200 ::
-    8201 ::
-    8202 ::
-    8239 ::
-    8287 ::
-    8288 :: (* <ZWNBSP> *)
-    12288 ::
-    []))
-  let digits: character list = to_character_list ('0' :: '1' :: '2' :: '3' :: '4' :: '5' :: '6' :: '7' :: '8' :: '9' :: [])
-  let ascii_word_characters: character list = to_character_list (
-    let str = "ABCDEFGHIJKLMNOPQRSTUVWXYZabcdefghijklmnopqrstuvwxyz0123456789_" in
-    List.init (String.length str) (String.get str))
-
-  let case_fold (c: character): character = 
-    if (Uchar.is_valid c) then
-      match Uucp.Case.Fold.fold (Uchar.of_int c) with
-        | `Self -> c
-        | `Uchars (cp :: []) -> Uchar.to_int cp
-        | `Uchars _ -> c
-    else c
-
+module UnicodeProperties = struct
   type unicodeProperty = 
   | Predicate of string
 
@@ -213,10 +54,76 @@ module Unicode = struct
     if (Uchar.is_valid c) then f (Uchar.of_int c)
     else d
 
-  let code_points_for up =
+  let filter_for up =
     let f = char_adapter false (match up with
     | Predicate "Alphabetic" -> Uucp.Alpha.is_alphabetic
     | Predicate name -> failwith ("Unknown property: " ^ name))
     in
-    List.filter f all_chars
+    List.filter f
+end
+
+module type InteropSig = sig
+  include Encoding.Character
+  val max: int
+  type property
+end
+
+module Interop (I: InteropSig) = struct
+  include I
+
+  let to_character_list (ls: char list): character list = List.map (fun c -> char_from_int (Char.code c)) ls
+  let all_chars: character list = 
+      List.init (max + 1) char_from_int
+
+  let line_terminators: character list = (List.map char_from_int Common.line_terminators)
+  let white_spaces: character list = (List.map char_from_int Common.white_spaces)
+  let digits: character list = to_character_list Common.digits
+  let ascii_word_characters: character list = to_character_list Common.ascii_word_characters
+end
+
+module Utf16Sig : InteropSig
+  with type character = Unsigned.uint16
+  with type property = unit
+= struct
+  include Encoding.Utf16
+  let max: int = Unsigned.UInt16.to_int Unsigned.UInt16.max_int
+  type property = unit
+end
+
+module UnicodeSig : InteropSig
+  with type character = int
+  with type property = UnicodeProperties.unicodeProperty
+= struct
+  include Encoding.Unicode
+  let max: int = 0x10FFFF
+  type property = UnicodeProperties.unicodeProperty
+end
+
+module Utf16 = struct
+  module Base = Interop(Utf16Sig)
+  include Base
+
+  let code_points_to_string (c: Encoding.codepoint list): character list = List.flatten (List.map chars_from_int c)
+
+  let to_upper_case (c: Encoding.codepoint): Encoding.codepoint list =
+    if Uchar.is_valid c then
+      match Uucp.Case.Map.to_upper (Uchar.of_int c) with
+        | `Self -> c :: []
+        | `Uchars ls -> List.map Uchar.to_int ls
+    else c :: []
+end
+
+module Unicode = struct
+  module Base = Interop(UnicodeSig)
+  include Base
+
+  let case_fold (c: character): character = 
+    if (Uchar.is_valid c) then
+      match Uucp.Case.Fold.fold (Uchar.of_int c) with
+        | `Self -> c
+        | `Uchars (cp :: []) -> Uchar.to_int cp
+        | `Uchars _ -> c
+    else c
+
+  let code_points_for_property up = UnicodeProperties.filter_for up all_chars
 end
