extraction/Notations.ml
@@ -1,37 +1,54 @@
+(** Defines notations to define regexes
+    You should either import Utf16Notations or UnicodeNotations    
+*)
 open Extracted.Patterns
-open Interop.Unicode
 
-let epsilon = Empty
-let char c =
-  match Interop.Utf16.string_to_utf16 c with
-  | h :: [] -> Char (Obj.magic h)
-  | _ -> failwith (String.cat "Invalid character: " c)
-let achar c = Char (Obj.magic (Interop.Utf16.char_of_int (Char.code c)))
-let sc c = SourceCharacter (Obj.magic (Interop.Utf16.char_of_int (Char.code c)))
-let uprop n = AtomEsc (ACharacterClassEsc (UnicodeProp (Obj.magic (Predicate n))))
+module CharNotations (S: Encoding.Character) = struct
+  type character = S.character
 
-let group r = Group (None, r)
-let ngroup p = Group (Some (fst p), (snd p))
+  let epsilon = Empty
+  let group r = Group (None, r)
+  let ngroup p = Group (Some (fst p), (snd p))
 
-(* let uprop name = AtomEsc (ACharacterClassEsc (UnicodeProp (Obj.magic ))) *)
+  let (||) l r = Disjunction (l, r)
 
-let (||) l r = Disjunction (l, r)
+  let (!*) r = Quantified (r, Greedy Star)
+  let (!*?) r = Quantified (r, Lazy Star)
 
-let (!*) r = Quantified (r, Greedy Star)
-let (!*?) r = Quantified (r, Lazy Star)
+  let (!+) r = Quantified (r, Greedy Plus)
+  let (!+?) r = Quantified (r, Lazy Plus)
 
-let (!+) r = Quantified (r, Greedy Plus)
-let (!+?) r = Quantified (r, Lazy Plus)
+  let (!?) r = Quantified (r, Greedy Question)
+  let (!??) r = Quantified (r, Lazy Question)
 
-let (!?) r = Quantified (r, Greedy Question)
-let (!??) r = Quantified (r, Lazy Question)
+  let (--) r1 r2 = Seq (r1, r2)
 
-let (--) r1 r2 = Seq (r1, r2)
+  let (?=) r = Lookahead r
+  let (?<=) r = Lookbehind r
+  let (?!) r = NegativeLookahead r
+  let (?<!) r = NegativeLookbehind r
 
-let (?=) r = Lookahead r
-let (?<=) r = Lookbehind r
-let (?!) r = NegativeLookahead r
-let (?<!) r = NegativeLookbehind r
+  let (!$) n = assert(0 < n); AtomEsc (DecimalEsc n)
+  let (!&) n = AtomEsc (GroupEsc n)
 
-let (!$) n = assert(0 < n); AtomEsc (DecimalEsc n)
-let (!&) n = AtomEsc (GroupEsc n)
+  let lchar (c: character list): character coq_Regex =
+    match c with
+    | h :: [] -> Char h
+    | _ -> failwith (String.cat "Invalid character: " (S.list_to_string c))
+
+  let char (c: string): character coq_Regex = lchar (S.list_from_string c)
+
+  let ichar (c: int): character coq_Regex = lchar (S.chars_from_int c)
+
+  let cchar (c: char): character coq_Regex = ichar (Char.code c)
+
+  let sc c = SourceCharacter (S.char_from_int (Char.code c))
+end
+
+module Utf16Notations = CharNotations(Encoding.Utf16)
+module UnicodeNotations = struct
+  module Base = CharNotations(Encoding.Unicode)
+  include Base
+
+  let uprop n = AtomEsc (ACharacterClassEsc (UnicodeProp (Obj.magic (Interop.UnicodeProperties.Predicate n))))
+end
