extraction/Testing.ml
@@ -1,0 +1,77 @@
+open Engines
+
+module Tester (E: Engine) = struct
+  include E
+  open Extracted.Notation
+
+  let pretty_print_result ls_input at (res: character coq_MatchResult) unicode =
+    let input = list_to_string ls_input in
+    match res with
+    | Success (Some { MatchState.endIndex = i; MatchState.captures = captures; MatchState.input = _ }) -> 
+      Printf.printf "Matched %d characters ([%d-%d]) in '%s' (length=%d)\n" (i - at) at i input (List.length ls_input);
+      let f id = 
+        match List.nth captures (id - 1) with
+        | None ->
+            Printf.printf "Group %d: undefined\n" id
+        | Some { CaptureRange.startIndex = s; CaptureRange.endIndex = e } ->
+            Printf.printf "Group %d: '%s' ([%d-%d])\n" id (list_to_string (Utils.List.sublist ls_input s e)) s e
+      in
+      List.iter f (Extracted.List.Range.Nat.Length.range 1 (List.length captures))
+
+    | Success None -> Printf.printf "No match on '%s' \n" input
+
+    | Failure OutOfFuel -> Printf.printf "Out of fuel on '%s' \n" input
+
+    | Failure AssertionFailed -> Printf.printf "Assertion error during matching on '%s' \n" input
+
+  let test_regex_using_record regex input at rer =
+    match compilePattern regex rer with
+    | Success matcher ->
+      let ls_input = list_from_string input in
+      pretty_print_result ls_input at (matcher ls_input at) true
+      
+    | Failure AssertionFailed -> Printf.printf "Assertion error during compilation \n"
+
+
+  let test_regex regex input at ?(ignoreCase=false) ?(multiline=false) ?(dotAll=false) ?(unicode=false) () =
+    let groups = (countGroups regex) in
+    let rer = Extracted.({
+      RegExpRecord.ignoreCase = ignoreCase;
+      RegExpRecord.multiline = multiline;
+      RegExpRecord.dotAll = dotAll;
+      RegExpRecord.unicode = unicode;
+      RegExpRecord.capturingGroupsCount = groups;
+    }) in
+    test_regex_using_record regex input at rer
+
+  let compare_regexes_using_record regex1 regex2 input at rer: unit =
+    match compilePattern regex1 rer, compilePattern regex2 rer with
+    | Success m1, Success m2 ->
+      let ls_input = list_from_string input in
+      let res1 = (m1 ls_input at) in
+      let res2 = (m2 ls_input at) in
+      if res1 = res2 then
+        (Printf.printf "The two regexes resulted in identical matches.\n";
+        pretty_print_result ls_input at res1 true)
+      else
+        (Printf.printf "The two regexes resulted in different matches.\n";
+        pretty_print_result ls_input at res1 true;
+        pretty_print_result ls_input at res2 true)
+
+    | Failure AssertionFailed, _ -> Printf.printf "Assertion error during compilation \n"
+    | _, Failure AssertionFailed -> Printf.printf "Assertion error during compilation \n"
+
+  let compare_regexes r1 r2 input at ?(ignoreCase=false) ?(multiline=false) ?(dotAll=false) ?(unicode=false) () =
+    let groups = (countGroups r1) in
+    let rer = Extracted.({
+      RegExpRecord.ignoreCase = ignoreCase;
+      RegExpRecord.multiline = multiline;
+      RegExpRecord.dotAll = dotAll;
+      RegExpRecord.unicode = unicode;
+      RegExpRecord.capturingGroupsCount = groups;
+    }) in
+    compare_regexes_using_record r1 r2 input at rer
+end
+
+module Utf16Tester = Tester(Engines.Utf16Engine)
+module UnicodeTester = Tester(Engines.UnicodeEngine)
