extraction/Utils.ml
@@ -1,0 +1,26 @@
+module List = struct
+  let rec drop n ls = 
+    if n <= 0 then
+      ls
+    else
+      match ls with
+      | _ :: ls' -> drop (n-1) ls'
+      | [] -> []
+
+  let rec take n ls = 
+    if n <= 0 then
+      []
+    else
+      match ls with
+      | h :: ls' -> h :: (take (n-1) ls')
+      | [] -> []
+
+  let sublist ls s e = take (e - s) (drop s ls)
+
+  let flat_map (type a b) (f: a -> b list) (ls: a list): b list =
+    List.flatten (List.map f ls)
+
+  let unique (type a) (ls: a list) = match ls with
+    | h :: [] -> h
+    | _ -> failwith "List is not a singleton"
+end
