test/BoundaryAssertions.ml
@@ -1,24 +1,24 @@
-open! Warblre.Extracted.Patterns
-open Warblre.Helpers
-open Warblre.Notations
+open Warblre.Notations.UnicodeNotations
+open Warblre.Testing.UnicodeTester
+
 
 let%expect_test "match_start_pos" =
   test_regex
-    (InputStart -- achar 'a')
+    (InputStart -- cchar 'a')
     "aa"
     0 ();
   [%expect {| Matched 1 characters ([0-1]) in 'aa' (length=2) |}]
 
 let%expect_test "match_start_neg_0" =
   test_regex
-    (InputStart -- achar 'a')
+    (InputStart -- cchar 'a')
     "aa"
     1 ();
   [%expect {| No match on 'aa' |}]
 
 let%expect_test "match_start_neg_1" =
   test_regex
-    ((achar 'a') -- InputStart -- (achar 'a'))
+    ((cchar 'a') -- InputStart -- (cchar 'a'))
     "aa"
     0 ();
   [%expect {| No match on 'aa' |}]
@@ -27,21 +27,21 @@ let%expect_test "match_start_neg_1" =
 
 let%expect_test "match_end_pos" =
   test_regex
-    ((achar 'a') -- InputEnd)
+    ((cchar 'a') -- InputEnd)
     "aa"
     1 ();
   [%expect {| Matched 1 characters ([1-2]) in 'aa' (length=2) |}]
 
 let%expect_test "match_start_neg_0" =
   test_regex
-  ((achar 'a') -- InputEnd)
+  ((cchar 'a') -- InputEnd)
     "aa"
     0 ();
   [%expect {| No match on 'aa' |}]
 
 let%expect_test "match_start_neg_1" =
   test_regex
-    ((achar 'a') -- InputEnd -- (achar 'a'))
+    ((cchar 'a') -- InputEnd -- (cchar 'a'))
     "aa"
     0 ();
   [%expect {| No match on 'aa' |}]
@@ -50,14 +50,14 @@ let%expect_test "match_start_neg_1" =
 
   let%expect_test "word_boundary_pos" =
   test_regex
-    ((achar 'a') -- WordBoundary -- (achar ' '))
+    ((cchar 'a') -- WordBoundary -- (cchar ' '))
     "a a"
     0 ();
   [%expect {| Matched 2 characters ([0-2]) in 'a a' (length=3) |}]
 
 let%expect_test "word_boundary_neg" =
   test_regex
-    ((achar 'a') -- WordBoundary -- (achar 'a'))
+    ((cchar 'a') -- WordBoundary -- (cchar 'a'))
     "aaa"
     0 ();
   [%expect {| No match on 'aaa' |}]
@@ -66,14 +66,14 @@ let%expect_test "word_boundary_neg" =
 
 let%expect_test "not_word_boundary_pos" =
   test_regex
-    ((achar 'a') -- NotWordBoundary -- (achar 'a'))
+    ((cchar 'a') -- NotWordBoundary -- (cchar 'a'))
     "aaa"
     0 ();
   [%expect {| Matched 2 characters ([0-2]) in 'aaa' (length=3) |}]
 
 let%expect_test "not_word_boundary_neg" =
   test_regex
-    ((achar 'a') -- NotWordBoundary -- (achar ' '))
+    ((cchar 'a') -- NotWordBoundary -- (cchar ' '))
     "a a"
     0 ();
   [%expect {| No match on 'a a' |}]
