test/Lookarounds.ml
@@ -1,24 +1,23 @@
-open! Warblre.Extracted.Patterns
-open Warblre.Helpers
-open Warblre.Notations
+open Warblre.Notations.UnicodeNotations
+open Warblre.Testing.UnicodeTester
 
 let%expect_test "lookahead_0_pos" =
   test_regex
-    (achar 'a' -- (?= (achar 'b')))
+    (cchar 'a' -- (?= (cchar 'b')))
     "ab"
     0 ();
   [%expect {| Matched 1 characters ([0-1]) in 'ab' (length=2) |}]
 
 let%expect_test "lookahead_0_neg_0" =
   test_regex
-    (achar 'a' -- (?= (achar 'b')))
+    (cchar 'a' -- (?= (cchar 'b')))
     "a"
     0 ();
   [%expect {| No match on 'a' |}]
 
 let%expect_test "lookahead_0_neg_1" =
   test_regex
-    (achar 'a' -- (?= (achar 'b')))
+    (cchar 'a' -- (?= (cchar 'b')))
     "aa"
     0 ();
   [%expect {| No match on 'aa' |}]
@@ -26,21 +25,21 @@ let%expect_test "lookahead_0_neg_1" =
 
 let%expect_test "lookbehind_0_pos" =
   test_regex
-    ((?<= (achar 'a')) -- achar 'b')
+    ((?<= (cchar 'a')) -- cchar 'b')
     "ab"
     1 ();
   [%expect {| Matched 1 characters ([1-2]) in 'ab' (length=2) |}]
 
 let%expect_test "lookbehind_0_neg_0" =
   test_regex
-    ((?<= (achar 'a')) -- achar 'b')
+    ((?<= (cchar 'a')) -- cchar 'b')
     "b"
     0 ();
   [%expect {| No match on 'b' |}]
 
 let%expect_test "lookbehind_0_neg_1" =
   test_regex
-    ((?<= (achar 'a')) -- achar 'b')
+    ((?<= (cchar 'a')) -- cchar 'b')
     "bb"
     1 ();
   [%expect {| No match on 'bb' |}]
@@ -49,21 +48,21 @@ let%expect_test "lookbehind_0_neg_1" =
 
 let%expect_test "neglookahead_0_pos_0" =
   test_regex
-    (achar 'a' -- (?! (achar 'b')))
+    (cchar 'a' -- (?! (cchar 'b')))
     "aa"
     0 ();
   [%expect {| Matched 1 characters ([0-1]) in 'aa' (length=2) |}]
 
 let%expect_test "neglookahead_0_pos_1" =
   test_regex
-    (achar 'a' -- (?! (achar 'b')))
+    (cchar 'a' -- (?! (cchar 'b')))
     "a"
     0 ();
   [%expect {| Matched 1 characters ([0-1]) in 'a' (length=1) |}]
 
 let%expect_test "neglookahead_0_neg" =
   test_regex
-    (achar 'a' -- (?! (achar 'b')))
+    (cchar 'a' -- (?! (cchar 'b')))
     "ab"
     0 ();
   [%expect {| No match on 'ab' |}]
@@ -71,21 +70,21 @@ let%expect_test "neglookahead_0_neg" =
 
 let%expect_test "neglookbehind_0_pos_0" =
   test_regex
-    ((?<! (achar 'a')) -- achar 'b')
+    ((?<! (cchar 'a')) -- cchar 'b')
     "bb"
     1 ();
   [%expect {| Matched 1 characters ([1-2]) in 'bb' (length=2) |}]
 
 let%expect_test "neglookbehind_0_pos_1" =
   test_regex
-    ((?<! (achar 'a')) -- achar 'b')
+    ((?<! (cchar 'a')) -- cchar 'b')
     "b"
     0 ();
   [%expect {| Matched 1 characters ([0-1]) in 'b' (length=1) |}]
 
 let%expect_test "neglookbehind_0_neg" =
   test_regex
-    ((?<! (achar 'a')) -- achar 'b')
+    ((?<! (cchar 'a')) -- cchar 'b')
     "ab"
     1 ();
   [%expect {| No match on 'ab' |}]
@@ -94,35 +93,35 @@ let%expect_test "neglookbehind_0_neg" =
 (* Note: using [^]  would be better than . *)
 let%expect_test "lookbehind_anchor_emulation_pos_0" =
   test_regex
-    ((?<! (Dot)) -- !*(achar 'b'))
+    ((?<! (Dot)) -- !*(cchar 'b'))
     "bbbb"
     0 ();
   [%expect {| Matched 4 characters ([0-4]) in 'bbbb' (length=4) |}]
 
   let%expect_test "lookbehind_anchor_emulation_neg_0" =
   test_regex
-    ((?<! (Dot)) -- !*(achar 'b'))
+    ((?<! (Dot)) -- !*(cchar 'b'))
     "bbbb"
     1 ();
   [%expect {| No match on 'bbbb' |}]
 
 let%expect_test "lookbehind_anchor_emulation_neg_1" =
   test_regex
-    ((?<! (Dot)) -- !*(achar 'b'))
+    ((?<! (Dot)) -- !*(cchar 'b'))
     "abbbb"
     1 ();
   [%expect {| No match on 'abbbb' |}]
 
 let%expect_test "lookahead_anchor_emulation_pos_0" =
   test_regex
-    (!*(achar 'b') -- (?! (Dot)))
+    (!*(cchar 'b') -- (?! (Dot)))
     "bbbb"
     0 ();
   [%expect {| Matched 4 characters ([0-4]) in 'bbbb' (length=4) |}]
 
 let%expect_test "lookbehind_anchor_emulation_neg_0" =
   test_regex
-    (!*(achar 'b') -- (?! (Dot)))
+    (!*(cchar 'b') -- (?! (Dot)))
     "bbbba"
     0 ();
   [%expect {| No match on 'bbbba' |}]
