extraction/Extraction.v
@@ -11,7 +11,7 @@ From Coq Require extraction.ExtrOcamlZInt.
 Extract Constant Pos.to_nat => "(fun c -> c)".
 
 Extract Constant HexDigit.type => "char".
-Extract Constant HexDigit.to_integer => "Interop.parse_hex".
+Extract Constant HexDigit.to_integer => "Interop.Common.parse_hex".
 
 Extract Constant AsciiLetter.type => "char".
 Extract Constant AsciiLetter.numeric_value => "Char.code".
@@ -21,12 +21,12 @@ Extract Constant Patterns.GroupName_eq_dec => "String.equal".
 
 Extract Constant UInt16.code_points_to_string => "Interop.Utf16.code_points_to_string".
 Extract Constant UInt16.to_upper_case => "Interop.Utf16.to_upper_case".
-Extract Constant UInt16.type => "Interop.Utf16.character".
-Extract Constant UInt16.to_code_point => "Interop.Utf16.code_point".
-Extract Constant UInt16.CodePoint => "Interop.Utf16.codepoint".
-Extract Constant UInt16.numeric_value => "Interop.Utf16.char_to_int".
-Extract Constant UInt16.from_numeric_value => "Interop.Utf16.char_of_int".
-Extract Constant UInt16.compare => "Interop.Utf16.cmp".
+Extract Constant UInt16.type => "Encoding.Utf16.character".
+Extract Constant UInt16.to_code_point => "Encoding.Utf16.char_to_int".
+Extract Constant UInt16.CodePoint => "Encoding.codepoint".
+Extract Constant UInt16.numeric_value => "Encoding.Utf16.char_to_int".
+Extract Constant UInt16.from_numeric_value => "Encoding.Utf16.char_from_int".
+Extract Constant UInt16.compare => "Encoding.Utf16.cmp".
 
 Extract Constant UInt16.all => "Interop.Utf16.all_chars".
 Extract Constant UInt16.line_terminators => "Interop.Utf16.line_terminators".
@@ -35,10 +35,10 @@ Extract Constant UInt16.digits => "Interop.Utf16.digits".
 Extract Constant UInt16.ascii_word_characters => "Interop.Utf16.ascii_word_characters".
 
 
-Extract Constant Unicode.type => "Interop.Unicode.character".
-Extract Constant Unicode.numeric_value => "Interop.Unicode.char_to_int".
-Extract Constant Unicode.from_numeric_value => "Interop.Unicode.char_of_int".
-Extract Constant Unicode.compare => "Interop.Unicode.cmp".
+Extract Constant Unicode.type => "Encoding.Unicode.character".
+Extract Constant Unicode.numeric_value => "Encoding.Unicode.char_to_int".
+Extract Constant Unicode.from_numeric_value => "Encoding.Unicode.char_from_int".
+Extract Constant Unicode.compare => "Encoding.Unicode.cmp".
 Extract Constant Unicode.case_fold => "Interop.Unicode.case_fold".
 
 Extract Constant Unicode.all => "Interop.Unicode.all_chars".
@@ -47,9 +47,9 @@ Extract Constant Unicode.white_spaces => "Interop.Unicode.white_spaces".
 Extract Constant Unicode.digits => "Interop.Unicode.digits".
 Extract Constant Unicode.ascii_word_characters => "Interop.Unicode.ascii_word_characters".
 
-Extract Constant Unicode.UnicodeProperty => "Interop.Unicode.unicodeProperty".
-Extract Constant Unicode.unicode_property_eqdec => "Interop.Unicode.up_eq".
-Extract Constant Unicode.code_points_for => "Interop.Unicode.code_points_for".
+Extract Constant Unicode.UnicodeProperty => "Interop.UnicodeProperties.unicodeProperty".
+Extract Constant Unicode.unicode_property_eqdec => "Interop.UnicodeProperties.up_eq".
+Extract Constant Unicode.code_points_for => "Interop.Unicode.code_points_for_property".
 
-Extraction "Extracted.ml" RegExpRecord.RegExpRecord  ECMA.ECMA ECMA.ECMA_u.
+Extraction "Extracted.ml"  ECMA.ECMA ECMA.ECMA_u.
 
